Strata/Languages/C_Simp/DDMTransform/Translate.lean
@@ -269,19 +269,14 @@ partial def translateExprs (bindings : TransBindings) (args : Array Arg) :
 end
 
 def translateMeasure (bindings : TransBindings) (arg : Arg) :
-    TransM (Option (String × LExpr CSimpLParams.mono)) := do
+    TransM (Option (LExpr CSimpLParams.mono)) := do
   translateOption (fun maybe_arg => do
                     match maybe_arg with
                     | none => return none
                     | some a =>
                       let e ← checkOpArg a q`C_Simp.measure 1
                       assert! e.size == 1
-                      let fname :=
-                        if bindings.currentFunction.isEmpty then "anon"
-                        else bindings.currentFunction
-                      let sr := a.ann
-                      let label := s!"{fname}_measure_{sr.start}_{sr.stop}"
-                      return some (label, ← translateExpr bindings e[0]!))
+                      return some (← translateExpr bindings e[0]!))
                   arg
 
 def translateInvariant (bindings : TransBindings) (arg : Arg) :
