StrataTest/DL/Imperative/FormatStmtTest.lean
@@ -145,7 +145,7 @@ info: while
 }
 -/
 #guard_msgs in
-#eval! format (Stmt.loop (.det xEq0) (some ("", x)) [("inv1", tt)]
+#eval! format (Stmt.loop (.det xEq0) (some x) [("inv1", tt)]
                 ([Statement.set "x" int1 .empty] : Ss) .empty : S)
 
 -- 14. exit with label
