StrataTest/Languages/C_Simp/Examples/LinearSearch.lean
@@ -69,7 +69,7 @@ info: function linearSearch {
   idx := #0
   while
     (~Int.Lt idx (~Array.Len arr))
-    ([linearSearch_measure_437_464]: (~Int.Sub (~Array.Len arr) idx))
+    ((~Int.Sub (~Array.Len arr) idx))
     [[linearSearch_invariant_467_484]: #true]
   {
     if (e == (~Array.Get arr idx)) {
